ReTierProofAggregation.v
@@ -1,31 +1,29 @@
 Require Import ReTierSyntax.
 Require Import ReTierStaticSemantics.
 Require Import ReTierDynamicSemantics.
+Require Import ReTierProofTransmission.
 
 Lemma aggregation_multiple:
-  forall program Psi Delta Gamma P P0 P1 peers v v_agg v_type,
+  forall program Psi Delta Delta' Gamma Gamma' P0 P1 peers v v_agg v_type,
+  peers_tied program P0 P1 ->
   peer_ties program (P0, P1) = Multiple ->
   value v ->
   transmittable_type v_type ->
-  program :: Psi; Delta; Gamma; P |- v : v_type ->
+  List.incl peers (peer_instances_of_type program P1) ->
+  program :: Psi; Delta; Gamma; P1 |- v : v_type ->
   Phi (peer_ties program) P0 P1 peers v v_type = Some v_agg ->
-    value v_agg /\
-    transmittable_type (List v_type) /\
-    program :: Psi; Delta; Gamma; P |- v_agg : List v_type.
+  program :: Psi; Delta'; Gamma'; P0 |- v_agg : List v_type.
 Proof.
 intros until v_type.
-intros H_multiple H_value H_transmittable H_type H_Phi.
+intros H_tied H_multiple H_value H_transmittable H_instances H_type H_Phi.
 generalize dependent v_agg.
 induction peers as [| peer0 peers IH_peers ]; intros v_agg H_Phi.
 - simpl in H_Phi.
   rewrite H_multiple in H_Phi.
   inversion H_Phi.
-  repeat split.
-  + apply v_nil.
-  + apply U_List. assumption.
-  + apply T_Nil.
+  apply T_Nil.
 - assert (H : exists v_agg, Phi (peer_ties program) P0 P1 peers v v_type = Some v_agg).
-  + clear IH_peers H_Phi.
+  + clear IH_peers H_instances H_Phi.
     induction peers as [| peer1 peers IH_peers ].
     * simpl.
       rewrite H_multiple.
@@ -33,9 +31,9 @@ induction peers as [| peer0 peers IH_peers ]; intros v_agg H_Phi.
       reflexivity.
     * simpl.
       rewrite H_multiple.
-      inversion IH_peers as [ v_agg2 H_Phi2 ].
-      rewrite H_Phi2.
-      exists (cons v v_agg2).
+      destruct IH_peers as [ v_agg2 H_Phi ].
+      rewrite H_Phi.
+      esplit.
       reflexivity.
   + inversion H as [ v_agg2 H_Phi2 ].
     simpl in H_Phi.
@@ -44,95 +42,91 @@ induction peers as [| peer0 peers IH_peers ]; intros v_agg H_Phi.
     rewrite H_Phi2 in IH_peers.
     clear H_Phi2.
     inversion H_Phi.
-    repeat split.
-    * apply v_cons; try assumption.
-      apply IH_peers.
-      reflexivity.
-    * apply U_List. assumption.
-    * apply T_Cons; try assumption.
-      apply IH_peers.
-      reflexivity.
+    apply T_Cons.
+    * eapply transmission; try eassumption.
+      unfold List.incl.
+      intros.
+      simpl in H0.
+      destruct H0; try contradiction.
+      subst.
+      apply H_instances.
+      simpl.
+      left. reflexivity.
+    * apply IH_peers; try reflexivity.
+      unfold List.incl.
+      intros.
+      apply H_instances.
+      simpl.
+      right. assumption.
 Qed.
 
 Lemma aggregation_optional:
-  forall program Psi Delta Gamma P P0 P1 peers v v_agg v_type,
+  forall program Psi Delta Delta' Gamma Gamma' P0 P1 peers v v_agg v_type,
+  peers_tied program P0 P1 ->
   peer_ties program (P0, P1) = Optional ->
   value v ->
   transmittable_type v_type ->
-  program :: Psi; Delta; Gamma; P |- v : v_type ->
+  List.incl peers (peer_instances_of_type program P1) ->
+  program :: Psi; Delta; Gamma; P1 |- v : v_type ->
   Phi (peer_ties program) P0 P1 peers v v_type = Some v_agg ->
-    value v_agg /\
-    transmittable_type (Option v_type) /\
-    program :: Psi; Delta; Gamma; P |- v_agg : Option v_type.
+  program :: Psi; Delta'; Gamma'; P0 |- v_agg : Option v_type.
 Proof.
 intros until v_type.
-intros H_multiple H_value H_transmittable H_type H_Phi.
+intros H_tied H_optional H_value H_transmittable H_instances H_type H_Phi.
 destruct peers.
 - simpl in H_Phi.
-  rewrite H_multiple in H_Phi.
+  rewrite H_optional in H_Phi.
   inversion H_Phi.
-  repeat split.
-  + apply v_none.
-  + apply U_Option. assumption.
-  + apply T_None.
+  apply T_None.
 - simpl in H_Phi.
-  rewrite H_multiple in H_Phi.
+  rewrite H_optional in H_Phi.
   destruct peers.
   + inversion H_Phi.
-    repeat split.
-    * apply v_some. assumption.
-    * apply U_Option. assumption.
-    * apply T_Some. assumption.
-  + contradict H_Phi.
-    congruence.
+    apply T_Some.
+    eapply transmission; eassumption.
+  + congruence.
 Qed.
 
 Lemma aggregation_single:
-  forall program Psi Delta Gamma P P0 P1 peers v v_agg v_type,
+  forall program Psi Delta Delta' Gamma Gamma' P0 P1 peers v v_agg v_type,
+  peers_tied program P0 P1 ->
   peer_ties program (P0, P1) = Single ->
   value v ->
   transmittable_type v_type ->
-  program :: Psi; Delta; Gamma; P |- v : v_type ->
+  List.incl peers (peer_instances_of_type program P1) ->
+  program :: Psi; Delta; Gamma; P1 |- v : v_type ->
   Phi (peer_ties program) P0 P1 peers v v_type = Some v_agg ->
-    value v_agg /\
-    transmittable_type v_type /\
-    program :: Psi; Delta; Gamma; P |- v_agg : v_type.
+  program :: Psi; Delta'; Gamma'; P0 |- v_agg : v_type.
 Proof.
 intros until v_type.
-intros H_multiple H_value H_transmittable H_type H_Phi.
+intros H_tied H_single H_value H_transmittable H_instances H_type H_Phi.
 destruct peers.
 - simpl in H_Phi.
-  rewrite H_multiple in H_Phi.
-  contradict H_Phi.
+  rewrite H_single in H_Phi.
   congruence.
 - simpl in H_Phi.
-  rewrite H_multiple in H_Phi.
+  rewrite H_single in H_Phi.
   destruct peers.
   + inversion H_Phi.
-    subst.
-    repeat split; assumption.
-  + contradict H_Phi.
-    congruence.
+    eapply transmission; eassumption.
+  + congruence.
 Qed.
 
 Lemma aggregation:
-  forall program Psi Delta Gamma P P0 P1 peers v v_agg v_type v_agg_type,
+  forall program Psi Delta Delta' Gamma Gamma' P0 P1 peers v v_agg v_type v_agg_type,
   peers_tied program P0 P1 ->
   Phi (peer_ties program) P0 P1 peers v v_type = Some v_agg ->
   phi (peer_ties program) P0 P1 v_type = Some v_agg_type ->
   value v ->
   transmittable_type v_type ->
-  program :: Psi; Delta; Gamma; P |- v : v_type ->
-    value v_agg /\
-    transmittable_type v_agg_type /\
-    program :: Psi; Delta; Gamma; P |- v_agg : v_agg_type.
+  List.incl peers (peer_instances_of_type program P1) ->
+  program :: Psi; Delta; Gamma; P1 |- v : v_type ->
+  program :: Psi; Delta'; Gamma'; P0 |- v_agg : v_agg_type.
 Proof.
 intros until v_agg_type.
-intros H_tied H_Phi H_phi_type H_value H_transmittable H_type.
+intros H_tied H_Phi H_phi_type H_value H_transmittable H_instances H_type.
 unfold phi in H_phi_type.
-remember (peer_ties program (P0, P1)) as multiplicity eqn:H_tie.
-symmetry in H_tie.
-destruct multiplicity; inversion H_phi_type; subst.
+destruct (peer_ties program (P0, P1)) eqn: H_tie; inversion H_phi_type; subst.
 - eapply aggregation_multiple; eassumption.
 - eapply aggregation_optional; eassumption.
 - eapply aggregation_single; eassumption.
