ReTierProofTransmission.v
@@ -1,0 +1,47 @@
+Require Import ReTierSyntax.
+Require Import ReTierStaticSemantics.
+Require Import ReTierDynamicSemantics.
+
+Lemma transmission : forall program Psi Delta Delta' Gamma Gamma' P P' theta v T,
+  value v ->
+  transmittable_type T ->
+  peers_tied program P' P ->
+  List.incl theta (peer_instances_of_type program P) ->
+  program :: Psi; Delta; Gamma; P |- v : T ->
+  program :: Psi; Delta'; Gamma'; P' |- zeta P theta v T : T.
+Proof.
+intros until T.
+intros H_value H_transmittable H_tied H_instance H_typing.
+generalize dependent T.
+induction v; intros; inversion H_value; inversion H_typing; subst.
+- inversion H_transmittable.
+- apply T_Unit.
+- apply T_None.
+- inversion H_transmittable.
+  simpl.
+  apply T_Some.
+  apply IHv; assumption.
+- apply T_Nil.
+- inversion H_transmittable.
+  simpl.
+  apply T_Cons.
+  + apply IHv1; assumption.
+  + apply IHv2; assumption.
+- apply T_Peer. assumption.
+- destruct H7; subst.
+  + simpl.
+    apply T_Signal.
+    apply T_ComFrom with (T0 := Unit).
+    * inversion H_transmittable.
+      assumption.
+    * apply U_Unit.
+    * apply T_Unit.
+    * apply T_Now with (T0 := Signal T1); try (left; reflexivity).
+      apply T_Reactive with (T1 := T1); try (left; reflexivity).
+      assumption.
+    * assumption.
+    * apply T_Peer.
+      assumption.
+  + inversion H_transmittable.
+- apply T_Nat.
+Qed.
